hott/init/funext.lean
@@ -32,7 +32,7 @@ open eq is_trunc sigma function is_equiv equiv prod unit
   Π ⦃A : Type _⦄ {P : A → Type _} (f g : Πx, P x), (f ~ g) → f = g
 
 -- Weak funext says that a product of contractible types is contractible.
-@[hott, class] def weak_funext :=
+@[hott] def weak_funext :=
   Π ⦃A : Type _⦄ (P : A → Type _) [H: Πx, is_contr (P x)], is_contr (Πx, P x)
 
 @[hott] def weak_funext_of_naive_funext : naive_funext → weak_funext :=
@@ -95,24 +95,24 @@ end
 section
 
 -- local attribute weak_funext [reducible]
-@[hott] theorem funext_of_weak_funext (wf : weak_funext.{l k}) : funext.{l k} :=
+@[hott] def funext_of_weak_funext (wf : weak_funext.{l k}) : funext.{l k} :=
 begin
   intros A B f g,
-  let eq_to_f := λ h' x, f = g,
+  let eq_to_f := λ g' x, f = g',
   let sim2path := @homotopy_ind wf _ _ f eq_to_f idp,
   have t1 : sim2path f (homotopy.refl f) = idp,
-    from homotopy_ind_comp f eq_to_f idp,
+    by apply @homotopy_ind_comp wf,
   have t2 : apd10 (sim2path f (homotopy.refl f)) = (homotopy.refl f),
     from ap apd10 t1,
   have left_inv : apd10 ∘ (sim2path g) ~ id,
-    from (homotopy_ind f (λ g' x, apd10 (sim2path g' x) = x) t2) g,
-  have right_inv : (sim2path g) ∘ apd10 ~ id,
-    from (λ h, eq.rec_on h (homotopy_ind_comp f _ idp)),
+    from (@homotopy_ind wf _ _ f (λ g' x, apd10 (sim2path g' x) = x) t2) g,
+  have right_inv : @comp (f = g) (f ~ g) (f = g) (sim2path g) (@apd10 A B f g) ~ id,
+    {intro h, induction h, apply homotopy_ind_comp},
   exact is_equiv.adjointify apd10 (sim2path g) left_inv right_inv
 end
 
 @[hott] def funext_from_naive_funext : naive_funext → funext :=
-  comp funext_of_weak_funext weak_funext_of_naive_funext
+  funext_of_weak_funext ∘ weak_funext_of_naive_funext
 end
 
 section
@@ -122,35 +122,29 @@ section
     let w' := equiv.mk w H0 in
     let eqinv : A = B := ((@is_equiv.inv _ _ _ (univalence A B)) w') in
     let eq' := equiv_of_eq eqinv in
+    have eqretr : eq' = w', from (@right_inv _ _ (@equiv_of_eq A B) (univalence A B) w'),
+    have invs_eq : (to_fun eq')⁻¹ = (to_fun w')⁻¹, from inv_eq eq' w' eqretr,
     is_equiv.adjointify (@comp C A B w)
       (@comp C B A (is_equiv.inv w))
       (λ (x : C → B),
-        -- have eqretr : eq' = w',
-        --   from (@right_inv _ _ (@equiv_of_eq A B) (univalence A B) w'),
-        -- have invs_eq : (to_fun eq')⁻¹ = (to_fun w')⁻¹,
-        --   from inv_eq eq' w' eqretr,
-        -- have eqfin1 : Π(p : A = B), (to_fun (equiv_of_eq p)) ∘ ((to_fun (equiv_of_eq p))⁻¹ ∘ x) = x,
-        --   by intro p; induction p; reflexivity,
-        -- have eqfin : (to_fun eq') ∘ ((to_fun eq')⁻¹ ∘ x) = x,
-        --   from eqfin1 eqinv,
-        -- have eqfin' : (to_fun w') ∘ ((to_fun eq')⁻¹ ∘ x) = x,
-        --   from ap (λu, u ∘ _) eqretr⁻¹ ⬝ eqfin,
+        have eqfin1 : Π(p : A = B), (to_fun (equiv_of_eq p)) ∘ ((to_fun (equiv_of_eq p))⁻¹ ∘ x) = x,
+          by intro p; induction p; reflexivity,
+        have eqfin : (to_fun eq') ∘ ((to_fun eq')⁻¹ ∘ x) = x,
+          from eqfin1 eqinv,
+        have eqfin' : (to_fun w') ∘ ((to_fun eq')⁻¹ ∘ x) = x,
+          by { refine _ ⬝ eqfin, rwr eqretr },
         show (to_fun w') ∘ ((to_fun w')⁻¹ ∘ x) = x,
-          from ap (λu, _ ∘ (u ∘ _)) invs_eq⁻¹ ⬝ eqfin'
+          by { refine _ ⬝ eqfin', rwr invs_eq }
       )
       (λ (x : C → A),
-        -- have eqretr : eq' = w',
-        --   from (@right_inv _ _ (@equiv_of_eq A B) (univalence A B) w'),
-        -- have invs_eq : (to_fun eq')⁻¹ = (to_fun w')⁻¹,
-        --   from inv_eq eq' w' eqretr,
-        -- have eqfin1 : Π(p : A = B), (to_fun (equiv_of_eq p))⁻¹ ∘ ((to_fun (equiv_of_eq p)) ∘ x) = x,
-        --   by intro p; induction p; reflexivity,
-        -- have eqfin : (to_fun eq')⁻¹ ∘ ((to_fun eq') ∘ x) = x,
-        --   from eqfin1 eqinv,
-        -- have eqfin' : (to_fun eq')⁻¹ ∘ ((to_fun w') ∘ x) = x,
-        --   from ap (λu, _ ∘ (u ∘ _)) eqretr⁻¹ ⬝ eqfin,
+        have eqfin1 : Π(p : A = B), (to_fun (equiv_of_eq p))⁻¹ ∘ ((to_fun (equiv_of_eq p)) ∘ x) = x,
+          by intro p; induction p; reflexivity,
+        have eqfin : (to_fun eq')⁻¹ ∘ ((to_fun eq') ∘ x) = x,
+          from eqfin1 eqinv,
+        have eqfin' : (to_fun eq')⁻¹ ∘ ((to_fun w') ∘ x) = x,
+          by { refine _ ⬝ eqfin, rwr eqretr },
         show (to_fun w')⁻¹ ∘ ((to_fun w') ∘ x) = x,
-          from ap (λu, u ∘ _) invs_eq⁻¹ ⬝ eqfin'
+          by { refine _ ⬝ eqfin', rwr invs_eq }
       )
 
   -- We are ready to prove functional extensionality,
@@ -158,45 +152,45 @@ section
   @[hott] private def diagonal (B : Type _) : Type _
     := Σ xy : B × B, fst xy = snd xy
 
-  @[hott] private def isequiv_src_compose {A B : Type _}
+  @[hott] private def isequiv_src_compose {A : Type u} {B : Type v}
       : @is_equiv (A → diagonal B)
                  (A → B)
                  (comp (prod.fst ∘ sigma.fst)) :=
-    @ua_isequiv_postcompose _ _ _ (prod.fst ∘ sigma.fst)
+    @ua_isequiv_postcompose (diagonal B) _ _ (prod.fst ∘ sigma.fst)
         (is_equiv.adjointify (prod.fst ∘ sigma.fst)
           (λ x : B, (sigma.mk (x , x) idp : diagonal B)) (λx, idp)
           (λ ⟨⟨b, c⟩, p⟩, by { dsimp at p, induction p, refl }))
 
-  @[hott] private def isequiv_tgt_compose {A : Type _} {B : Type _}
+  @[hott] private def isequiv_tgt_compose {A : Type u} {B : Type v}
       : is_equiv (comp (prod.snd ∘ sigma.fst) : (A → diagonal B) → (A → B)) :=
-  begin
-    refine @ua_isequiv_postcompose _ _ _ (prod.snd ∘ sigma.fst) _,
+  @ua_isequiv_postcompose _ _ _ _ begin
     fapply adjointify,
     { intro b, exact ⟨(b, b), idp⟩},
     { intro b, reflexivity},
-    { intro a, induction a with q p, induction q, simp at *, induction p, reflexivity}
+    { intro a, induction a with q p, induction q, dsimp at *, induction p, reflexivity}
   end
 
   @[hott] theorem nondep_funext_from_ua {A : Type _} {B : Type _}
       : Π {f g : A → B}, f ~ g → f = g :=
-    (λ (f g : A → B) (p : f ~ g),
-        let d := λ (x : A), @sigma.mk (B × B) (λ (xy : B × B), xy.1 = xy.2) (f x , f x) (eq.refl (f x, f x).1) in
-        let e := λ (x : A), @sigma.mk (B × B) (λ (xy : B × B), xy.1 = xy.2) (f x , g x) (p x) in
-        let precomp1 := comp (sigma.fst ∘ sigma.fst) in
-        have equiv1 : is_equiv precomp1,
-          from @isequiv_src_compose A B,
-        have equiv2 : Π (x y : A → diagonal B), is_equiv (ap precomp1),
-          from is_equiv.is_equiv_ap precomp1,
-        have H' : Π (x y : A → diagonal B), sigma.fst ∘ prod.fst ∘ x = sigma.fst ∘ prod.fst ∘ y → x = y,
-          from (λ x y, is_equiv.inv (ap precomp1)),
-        have eq2 : sigma.fst ∘ prod.fst ∘ d = sigma.fst ∘ prod.fst ∘ e,
-          from idp,
-        have eq0 : d = e,
-          from H' d e eq2,
-        have eq1 : (sigma.snd ∘ prod.fst) ∘ d = (sigma.snd ∘ prod.fst) ∘ e,
-          from ap _ eq0,
-        eq1
-    )
+  begin
+    intros f g p,
+    let d := λ (x : A), @sigma.mk (B × B) (λ (xy : B × B), xy.1 = xy.2) (f x , f x) (eq.refl (f x, f x).1),
+    let e := λ (x : A), @sigma.mk (B × B) (λ (xy : B × B), xy.1 = xy.2) (f x , g x) (p x),
+    let precomp1 : (A → diagonal B) → (A → B) := comp (prod.fst ∘ sigma.fst),
+    have equiv1 : is_equiv precomp1,
+      from @isequiv_src_compose A B,
+    have equiv2 : Π (x y : A → diagonal B), is_equiv (ap precomp1),
+      from is_equiv.is_equiv_ap precomp1,
+    have H' : Π (x y : A → diagonal B), prod.fst ∘ sigma.fst ∘ x = prod.fst ∘ sigma.fst ∘ y → x = y,
+      from (λ x y, is_equiv.inv (ap precomp1)),
+    have eq2 : prod.fst ∘ sigma.fst ∘ d = prod.fst ∘ sigma.fst ∘ e,
+      from idp,
+    have eq0 : d = e,
+      from H' d e eq2,
+    have eq1 : (prod.snd ∘ sigma.fst) ∘ d = (prod.snd ∘ sigma.fst) ∘ e,
+      from ap _ eq0,
+    exact eq1
+  end
 
 end
 
@@ -257,6 +251,9 @@ namespace eq
   @[hott] def eq_of_homotopy_idp (f : Π x, P x) : eq_of_homotopy (λx : A, idpath (f x)) = idpath f :=
   is_equiv.left_inv apd10 idp
 
+  @[hott] def eq_of_homotopy_refl (f : Π x, P x) : eq_of_homotopy (homotopy.refl f) = idpath f :=
+  eq_of_homotopy_idp _
+
   @[hott] def naive_funext_of_ua : naive_funext :=
   λ A P f g h, eq_of_homotopy h
 
@@ -266,7 +263,7 @@ namespace eq
 
   @[hott] protected def homotopy.rec_on_idp {Q : Π{g}, (f ~ g) → Type _} {g : Π x, P x}
     (p : f ~ g) (H : Q (homotopy.refl f)) : Q p :=
-  homotopy.rec_on p (λq, eq.rec_on q H)
+  homotopy.rec_on p (λq, by induction q; exact H)
 
   @[hott] protected def homotopy.rec_on' {f f' : Πa, P a} {Q : (f ~ f') → (f = f') → Type _}
     (p : f ~ f') (H : Π(q : f = f'), Q (apd10 q) q) : Q p (eq_of_homotopy p) :=
@@ -275,7 +272,7 @@ namespace eq
     intro q, exact (left_inv (apd10) q)⁻¹ ▸ H q
   end
 
-  @[hott, elab_as_eliminator] protected def homotopy.rec_on_idp' {f : Πa, P a} {Q : Π{g}, (f ~ g) → (f = g) → Type _}
+  @[hott] protected def homotopy.rec_on_idp' {f : Πa, P a} {Q : Π{g}, (f ~ g) → (f = g) → Type _}
     {g : Πa, P a} (p : f ~ g) (H : Q (homotopy.refl f) idp) : Q p (eq_of_homotopy p) :=
   begin
     refine homotopy.rec_on' p _, intro q, induction q, exact H
@@ -285,21 +282,23 @@ namespace eq
     : eq_of_homotopy (λx, (H x)⁻¹ᵖ) = (eq_of_homotopy H)⁻¹ :=
   begin
     apply homotopy.rec_on_idp H,
-    rwr [eq_of_homotopy_idp]
+    change eq_of_homotopy (λ x, idp) = _,
+    rwr [eq_of_homotopy_refl],
   end
 
   @[hott] def eq_of_homotopy_con {f g h : Π x, P x} (H1 : f ~ g) (H2 : g ~ h)
     : eq_of_homotopy (λx, H1 x ⬝ H2 x) = eq_of_homotopy H1 ⬝ eq_of_homotopy H2 :=
   begin
-    apply homotopy.rec_on_idp H1,
-    apply homotopy.rec_on_idp H2,
-    rwr [eq_of_homotopy_idp]
+    apply homotopy.rec_on_idp H2; dsimp,
+    apply homotopy.rec_on_idp H1; dsimp,
+    rwr eq_of_homotopy_refl, apply eq_of_homotopy_idp,
   end
 
   @[hott] def compose_eq_of_homotopy {A B C : Type _} (g : B → C) {f f' : A → B} (H : f ~ f') :
     (ap (λf : A → B, g ∘ f) (eq_of_homotopy H): _) = eq_of_homotopy (hwhisker_left g H) :=
   begin
-    refine homotopy.rec_on_idp' H _, exact (eq_of_homotopy_idp _)⁻¹
+    apply homotopy.rec_on_idp H, rwr eq_of_homotopy_refl,
+    symmetry, apply eq_of_homotopy_idp
   end
 
 end eq
